theories/Signature.v
@@ -42,8 +42,10 @@ From Katamaran Require Export
 
 Module Type SignatureMixin
   (B : Base) (P : PredicateKit B) (W : WorldsMixin B P) (S : SolverKit B P W) :=
-  AssertionsOn B P W <+ UnifLogicOn B P W <+ SymPropOn B P W <+ LogSymPropOn B P W <+
-    GenericSolverOn B P W S <+ ShallowMonadsOn B P W <+ SymbolicMonadsOn B P W S <+
+  SymPropOn B P W <+ UnifLogicOn B P W <+ LogSymPropOn B P W  <+
+  AssertionsOn B P W <+
+    GenericSolverOn B P W S <+ ShallowMonadsOn B P W <+
+    SymbolicMonadsOn B P W S <+
     RefinementMonadsOn B P W S.
 
 Module Type Signature (B : Base) :=
