theories/Staging/WorldIsomorphisms.v
@@ -1,0 +1,282 @@
+(******************************************************************************)
+(* Copyright (c) 2020 Dominique Devriese, Georgy Lukyanov,                    *)
+(*   Sander Huyghebaert, Steven Keuchel                                       *)
+(* All rights reserved.                                                       *)
+(*                                                                            *)
+(* Redistribution and use in source and binary forms, with or without         *)
+(* modification, are permitted provided that the following conditions are     *)
+(* met:                                                                       *)
+(*                                                                            *)
+(* 1. Redistributions of source code must retain the above copyright notice,  *)
+(*    this list of conditions and the following disclaimer.                   *)
+(*                                                                            *)
+(* 2. Redistributions in binary form must reproduce the above copyright       *)
+(*    notice, this list of conditions and the following disclaimer in the     *)
+(*    documentation and/or other materials provided with the distribution.    *)
+(*                                                                            *)
+(* THIS SOFTWARE IS PROVIDED BY THE COPYRIGHT HOLDERS AND CONTRIBUTORS        *)
+(* "AS IS" AND ANY EXPRESS OR IMPLIED WARRANTIES, INCLUDING, BUT NOT LIMITED  *)
+(* TO, THE IMPLIED WARRANTIES OF MERCHANTABILITY AND FITNESS FOR A PARTICULAR *)
+(* PURPOSE ARE DISCLAIMED. IN NO EVENT SHALL THE COPYRIGHT HOLDER OR          *)
+(* CONTRIBUTORS BE LIABLE FOR ANY DIRECT, INDIRECT, INCIDENTAL, SPECIAL,      *)
+(* EXEMPLARY, OR CONSEQUENTIAL DAMAGES (INCLUDING, BUT NOT LIMITED TO,        *)
+(* PROCUREMENT OF SUBSTITUTE GOODS OR SERVICES; LOSS OF USE, DATA, OR         *)
+(* PROFITS; OR BUSINESS INTERRUPTION) HOWEVER CAUSED AND ON ANY THEORY OF     *)
+(* LIABILITY, WHETHER IN CONTRACT, STRICT LIABILITY, OR TORT (INCLUDING       *)
+(* NEGLIGENCE OR OTHERWISE) ARISING IN ANY WAY OUT OF THE USE OF THIS         *)
+(* SOFTWARE, EVEN IF ADVISED OF THE POSSIBILITY OF SUCH DAMAGE.               *)
+(******************************************************************************)
+
+From Coq Require Import
+  Classes.Morphisms
+  Classes.Morphisms_Prop
+  Classes.RelationClasses
+  Relations.Relation_Definitions
+.
+From Equations Require Import
+  Equations.
+From stdpp Require Import base.
+From Katamaran Require Import
+  Prelude
+  Base
+  Environment
+  Symbolic.Worlds
+  Symbolic.UnifLogic
+  Syntax.Predicates
+.
+From iris Require bi.derived_connectives bi.interface proofmode.tactics.
+
+Set Implicit Arguments.
+
+Module Type WorldIsomorphisms
+  (Import B : Base)
+  (Import P : PredicateKit B)
+  (Import W : WorldsMixin B P)
+  (Import UL : UnifLogicOn B P W).
+
+  Import ctx.notations.
+  Import ModalNotations.
+  Import iris.bi.interface.
+  Import iris.proofmode.tactics.
+
+
+  Definition Inverse {w1 w2 : World} (ω12 : Sub w1 w2) (ω21 : Sub w2 w1) :=
+    forall ι, instprop (wco w1) ι -> inst ω12 (inst ω21 ι) = ι.
+
+  Record IsIsomorphism {w1 w2 : World} (ω12 : Sub w1 w2) (ω21 : Sub w2 w1) :=
+    MkIsIsomorphism {
+        wiso_there : Inverse ω12 ω21
+      ; wiso_back : Inverse ω21 ω12
+      }.
+
+  Lemma iso_symm {w1 w2 : World} {ω12 : Sub w1 w2} {ω21 : Sub w2 w1} :
+    IsIsomorphism ω12 ω21 -> IsIsomorphism ω21 ω12.
+  Proof.
+    intros [Ht Hb].
+    now constructor.
+  Qed.
+
+  Lemma knowing_forgetting_iso {w1 w2 : World} {ω : Sub w1 w2} {ω' : Acc w2 w1} {P : Pred w1}
+    (H : IsIsomorphism ω (sub_acc ω')) :
+    P ⊣⊢ knowing ω (forgetting ω P).
+  Proof.
+    rewrite /forgetting /knowing.
+    crushPredEntails3.
+    - exists (inst (sub_acc ω') ι).
+      rewrite wiso_there; intuition.
+      now apply acc_pathcond.
+    - now subst.
+  Qed.
+
+  Lemma assuming_forgetting_inv {w1 w2 : World} {ω : Sub w1 w2} {ω' : Acc w2 w1} {P : Pred w1}
+    (inv : Inverse ω (sub_acc ω')) :
+    P ⊣⊢ assuming ω (forgetting ω P).
+  Proof.
+    rewrite /forgetting /assuming.
+    crushPredEntails3.
+    - now subst.
+    - specialize (H0 (inst (sub_acc ω') ι)).
+      rewrite inv in H0; intuition.
+      now apply H1, acc_pathcond.
+  Qed.
+
+  Lemma forgetting_knowing_iso {w1 w2 : World} {ω : Sub w1 w2} {ω' : Sub w2 w1} {P : Pred w2}
+    (inv : Inverse ω' ω) :
+    P ⊣⊢ forgetting ω (knowing ω P).
+  Proof.
+    rewrite /forgetting /knowing.
+    crushPredEntails3.
+    apply (f_equal (inst ω')) in H0.
+    rewrite !inv in H0; intuition.
+    now subst.
+  Qed.
+
+  Lemma knowing_knowing_iso {w1 w2 : World} {ω : Sub w1 w2} {ω' : Acc w2 w1} {P : Pred w1}
+    (inv : Inverse ω (sub_acc ω')) :
+    knowing ω (knowing (sub_acc ω') P) ⊣⊢ P.
+  Proof.
+    unfold knowing.
+    crushPredEntails3.
+    - subst.
+      now rewrite inv.
+    - exists (inst (sub_acc ω') ι).
+      repeat split.
+      + now apply inv.
+      + now apply acc_pathcond.
+      + now exists ι.
+  Qed.
+
+
+  Lemma forgetting_knowing_iso2 {w1 w2 : World} {ω : Acc w1 w2} {ω' : Acc w2 w1} {P : Pred w1}
+    (H : IsIsomorphism (sub_acc ω) (sub_acc ω')) :
+    knowing (sub_acc ω') P ⊣⊢ forgetting (sub_acc ω) P.
+  Proof.
+    rewrite (forgetting_knowing_iso (P := (knowing (sub_acc ω') P)) (wiso_back H)).
+    now rewrite (knowing_knowing_iso (wiso_there H)).
+  Qed.
+
+  Lemma assuming_assuming_inv {w1 w2 : World} {ω : Sub w1 w2} {ω' : Acc w2 w1} {P : Pred w1}
+    (iso : Inverse ω (sub_acc ω')) :
+    P ⊣⊢ assuming ω (assuming (sub_acc ω') P).
+  Proof.
+    rewrite /assuming.
+    crushPredEntails3; subst.
+    - now rewrite iso in H0.
+    - eapply H0; try easy.
+      + now apply iso.
+      + now apply acc_pathcond.
+  Qed.
+
+  Lemma forgetting_assuming_iso {w1 w2 : World} {ω : Sub w1 w2} {ω' : Sub w2 w1} {P : Pred w2}
+    (iso : Inverse ω' ω) :
+    P ⊣⊢ forgetting ω (assuming ω P).
+  Proof.
+    rewrite /forgetting /assuming.
+    crushPredEntails3.
+    apply (f_equal (inst ω')) in H1.
+    rewrite !iso in H1; intuition.
+    now subst.
+  Qed.
+
+  Lemma cancel_forgetting_iso {w1 w2 : World} {ω : Sub w1 w2} {ω' : Acc w2 w1} `{iso : IsIsomorphism ω (sub_acc ω')}
+    {P Q : Pred w1} :
+    (forgetting ω P ⊢ forgetting ω Q) -> P ⊢ Q.
+  Proof.
+    intros H.
+    rewrite (knowing_forgetting_iso (P := P) iso) (knowing_forgetting_iso (P := Q) iso).
+    now rewrite H.
+  Qed.
+
+  Lemma cancel_knowing_inv {w1 w2 : World} {ω : Acc w1 w2} {ω' : Acc w2 w1} `{inv : Inverse (sub_acc ω') (sub_acc ω)}
+    {P Q : Pred w2} :
+    (knowing (sub_acc ω) P ⊢ knowing (sub_acc ω) Q) -> P ⊢ Q.
+  Proof.
+    intros H.
+    rewrite (forgetting_knowing_iso (P := P) inv)
+      (forgetting_knowing_iso (P := Q) inv).
+    now rewrite H.
+  Qed.
+
+  Lemma forgetting_assuming_adjoint {w1 w2 : World} {ω : Acc w1 w2} {P Q} :
+    (forgetting (sub_acc ω) P ⊢ Q) <-> (P ⊢ assuming (sub_acc ω) Q).
+  Proof.
+    rewrite /forgetting /assuming.
+    split; crushPredEntails3.
+    - subst; now apply H4.
+    - apply (fromEntails H) with (inst (sub_acc ω) ι);
+        auto using acc_pathcond.
+  Qed.
+
+  Lemma forgetting_knowing_adjoint {w1 w2 : World} {ω : Acc w1 w2} {P Q} :
+    (knowing (sub_acc ω) P ⊢ Q) <-> (P ⊢ forgetting (sub_acc ω) Q).
+  Proof.
+    rewrite /forgetting /assuming /knowing.
+    split; crushPredEntails3.
+    - apply (fromEntails H); auto using acc_pathcond.
+      now exists ι.
+            - now subst.
+  Qed.
+
+  Lemma forgetting_knowing_adjoint_bientails_iso {w1 w2 : World} {ω : Acc w1 w2} {ω'} {P Q}
+    (iso : IsIsomorphism (sub_acc ω) (sub_acc ω')) :
+    (knowing (sub_acc ω) P ⊣⊢ Q) <-> (P ⊣⊢ forgetting (sub_acc ω) Q).
+  Proof.
+    rewrite /forgetting /assuming /knowing.
+    split; crushPredEntails3.
+    - apply (fromBientails H); auto using acc_pathcond.
+      now exists ι.
+            - destruct H as [H].
+              specialize  (H (inst (sub_acc ω) ι) (acc_pathcond ω ι H0)).
+              rewrite <-H in H1.
+              destruct H1 as (ι2 & eq & Hι2 & HP).
+              apply (f_equal (inst (sub_acc ω'))) in eq.
+              rewrite !(wiso_back iso) in eq; try assumption.
+              now subst.
+            - now subst.
+            - exists (inst (sub_acc ω') ι).
+              repeat split.
+              + now rewrite wiso_there.
+              + now apply acc_pathcond.
+              + apply (fromBientails H).
+                now apply acc_pathcond.
+                now rewrite wiso_there.
+  Qed.
+
+  Program Definition acc_let_right {w} (b : LVar ∷ Ty) v : w ⊒ wlet w b v :=
+    @acc_sub w (wlet w b v) sub_wk1 _.
+  Next Obligation.
+    intros * ι Hpc.
+    now apply proj1 in Hpc.
+  Defined.
+
+  Program Definition acc_let_left {w} (b : LVar ∷ Ty) v : wlet w b v ⊒ w :=
+    acc_sub (sub_snoc (sub_id w) b (term_val _ v)) _.
+  Next Obligation.
+    intros * ι Hpc.
+    split; last reflexivity.
+    change (subst_ctx ?pc ?ς)
+      with (subst pc ς).
+    now rewrite <-subst_sub_comp, sub_comp_wk1_tail, subst_sub_id.
+  Defined.
+
+  Program Definition acc_let_snoc {w} (b : LVar ∷ Ty) v : wsnoc w b ⊒ wlet w b v :=
+    acc_sub (sub_id (w ▻ b) : Sub (wsnoc w b) (wlet w b v)) _.
+  Next Obligation.
+    intros * ι.
+    destruct (env.view ι) as [ι v'].
+    unfold wlet; simpl.
+    intros Hpc.
+    destruct (proj1 (instprop_snoc _ _ _) Hpc) as [Hpc' H].
+    now rewrite instprop_subst inst_sub_id.
+  Defined.
+  
+  (* Lemma acc_let_iso w b v : IsIsomorphism (@acc_let_right w b v) (acc_let_left b v). *)
+  (* Proof. *)
+  (*   constructor; intros; simpl. *)
+  (*   - now rewrite inst_sub_snoc, inst_sub_id, inst_sub_wk1. *)
+  (*   - rewrite inst_sub_snoc, inst_sub_id. *)
+  (*     destruct (env.view ι) as (ι & v'). *)
+  (*     destruct H as (Hpc & Hbv); cbn in Hbv. *)
+  (*     subst. *)
+  (*     now rewrite inst_sub_wk1. *)
+  (* Qed. *)
+
+  (* Lemma assuming_acc_let_snoc {w b v P} : *)
+  (*   assuming (acc_let_left (w := w) b v) P ⊣⊢ (repₚ v term_var_zero -∗ forgetting acc_snoc_right P). *)
+  (* Proof. *)
+  (*   unfold assuming, forgetting, repₚ. *)
+  (*   crushPredEntails3; destruct (env.view ι) as [ι v']; subst; cbn in *. *)
+  (*   - rewrite instprop_subst inst_sub_wk1 in H; subst. *)
+  (*     crushPredEntails3. *)
+  (*     rewrite inst_sub_wk1. *)
+  (*     apply H0; try done. *)
+  (*     f_equal; try done. *)
+  (*     now apply inst_sub_id. *)
+  (*   - rewrite inst_sub_wk1 in H0. *)
+  (*     change (env.map _ _) with (inst (sub_id w) ιpast) in H1. *)
+  (*     rewrite inst_sub_id in H1. *)
+  (*     destruct (proj1 (env.inversion_eq_snoc ιpast ι v v') H1) as [-> ->]. *)
+  (*     now apply H0. *)
+  (* Qed. *)
+
+End WorldIsomorphisms.
