theories/Symbolic/Monads.v
@@ -38,6 +38,7 @@ From Katamaran Require Import
   Syntax.Chunks
   Syntax.Predicates
   Symbolic.Propositions
+  Symbolic.UnifLogic
   Symbolic.Solver
   Symbolic.Worlds.
 
@@ -47,8 +48,12 @@ Import env.notations.
 #[local] Set Implicit Arguments.
 
 Module Type SymbolicMonadsOn (Import B : Base) (Import P : PredicateKit B)
-  (Import W : WorldsMixin B P) (Import SK : SolverKit B P W)
-  (Import SP : SymPropOn B P W) (Import GS : GenericSolverOn B P W SK)
+  (Import W : WorldsMixin B P)
+  (Import SK : SolverKit B P W)
+  (Import SP : SymPropOn B P W)
+  (Import UL : UnifLogicOn B P W)
+  (Import LSP : LogSymPropOn B P W SP UL)
+  (Import GS : GenericSolverOn B P W SK SP UL LSP)
   (Import A : AssertionsOn B P W).
 
   Import ModalNotations.
